slightly dubious plan for splicing trees back together
this doesn't seem right; we have no frame predicate into which
we can conveniently fold away things as we run down the tree..
we should probably ask Adam what's the right pattern for this
kind of situation.

src/DirTree.v
@@ -420,6 +420,61 @@ Module DIRTREE.
     exact emp.
   Qed.
 
+
+  Definition dir_updater := dirtree -> dirtree.
+
+  Definition update_tree_helper (rec : dirtree -> dirtree) name
+                                (arg : string * addr * dir_item)
+                                (accum : dirtree) :=
+    let '(name', inum', item') := arg in
+    if string_dec name' name then
+    match item' with
+    | DirFile _ => arg :: accum
+    | DirSubdir tree' => (name', inum', DirSubdir (rec tree')) :: accum
+    end
+    else arg :: accum.
+
+  Fixpoint update_tree (fnlist : list string) (updater : dir_updater) (tree : dirtree) :=
+    match fnlist with
+    | nil => updater tree
+    | name :: rest =>
+      fold_right (update_tree_helper (update_tree rest updater) name) nil tree
+    end.
+
+  Definition add_to_dir (dir : dirtree) (name : string) (inum : addr) (newitem : dir_item) :=
+    (name, inum, newitem) :: dir.
+
+  Fixpoint delete_from_dir (dir : dirtree) (name : string) :=
+    match dir with
+    | nil => nil
+    | hd :: rest =>
+      let '(name', _, _) := hd in
+      if string_dec name' name then
+        delete_from_dir rest name
+      else
+        hd :: delete_from_dir rest name
+    end.
+
+
+  Theorem update_subtree : forall fsxp fnlist treetop m F Ftop itop
+                                  Fsub isub treesub
+                                  m' updater,
+    (F * rep fsxp Ftop itop treetop)%pred (list2mem m) ->
+    find_name fnlist treetop itop $1 = Some (isub, $1) ->
+    (F * rep fsxp Fsub isub treesub)%pred (list2mem m) ->
+    (F * rep fsxp Fsub isub (updater treesub))%pred (list2mem m') ->
+    (F * rep fsxp Ftop itop (update_tree fnlist updater treetop))%pred (list2mem m').
+  Proof.
+    induction fnlist; simpl.
+    intros.
+    inversion H0; subst. pred_apply. unfold rep. cancel. admit.
+    induction treetop; simpl; intros.
+    discriminate.
+    pred_apply. cancel.
+    admit.
+  Qed.
+
+
   Definition delete T fsxp dnum name mscs rx : prog T :=
     let^ (mscs, oi) <- SDIR.dslookup fsxp.(FSXPMemLog) fsxp.(FSXPBlockAlloc) fsxp.(FSXPInode)
                                      dnum name mscs;
